\subsection*{4.1} Prove the associative law of addition:

$$ (k+m) + n = k+(m+n)$$

\begin{proof}
Will prove by induction on $n$.

The base case is

$$ (k+m)+0 = k+m = k+(m+0)$$

, from the defining property of addition that $m+0=m$ for all $m$.

The inductive case is

\begin{align*}
    (k+m)+(n+1) &= ((k+m) + n) + 1 \\
                &= (k+(m+n)) + 1 \\
                &= k + ((m+n) + 1) \\
                &= k + (m+(n+1))
\end{align*}

, and hence the associativity proposition holds.

\end{proof}

