\subsection*{4.6} If $m, n, k \in N$ and $k > 0$, then $m < n$ if and only if $m \cdot k < n \cdot k$.

\begin{proof}
Assume that $m < n$. Will show by induction over $k$ that $m \cdot k < n \cdot k$.

For $k=1$, the proposition holds since $m \cdot 1 = (m \cdot 0) + m = m < n = (n \cdot 0) + n$.

Assuming that $m \cdot k < n \cdot k$, we have

$$m \cdot (k+1) = m \cdot k + m < n \cdot k + n = n \cdot (k+1)$$

, where we have used the property that $n < m$ iff $n + k < m + k$ for all $k \in N$ proved previously.

\end{proof}

