\subsection*{5.3} Simplify

\begin{itemize}
    \item $(\omega + 1) + \omega$
    \begin{proof}
        $$(\omega + 1) + \omega = \sup\{\omega + 1 + n | n < \omega\} = \sup\{\omega + n | n < \omega\} = \omega + \omega$$
    \end{proof}

    \item $\omega + \omega^2$
    
    \begin{proof}
        $$\omega + \omega^2 = \omega \cdot (1+\omega)= \omega \cdot \omega = \omega ^2$$
    \end{proof}

    \item $(\omega + 1) \cdot \omega ^2$

    \begin{proof}
      \begin{align*}
(\omega + 1) \cdot \omega ^2 = \sup\{(\omega + 1) \cdot n | n < \omega^2\} =\sup\{\omega \cdot n + (n+1) | n < \omega^2\} =\sup\{\omega \cdot n + n | n < \omega^2\}=\\ = \sup\{(\omega +1) \cdot n | n < \omega^2\} =
        (\omega+1) \cdot \omega^2 = \omega ^3+\omega^2
      \end{align*} 
    \end{proof}
\end{itemize}

