\subsection*{5.7b} For all ordinals $\alpha_1, \alpha_2$ and $\beta \neq 0$, $\beta \cdot \alpha_1 = \beta \cdot \alpha_2$ if and only if $\alpha_1 = \alpha_2$.

\begin{proof}
    Assume to the contrary that $\alpha_1 \neq \alpha_2$. Without loss of generalization, it follows that $\alpha_1 < \alpha_2$ and hence $\alpha_2 = \alpha_1 + \gamma$ for some $\gamma > 0$. Then, $\beta \cdot \alpha_1 = \beta \cdot \alpha_2$ is equivalent to $\beta \cdot \alpha_1 = \beta \cdot (\alpha_1 + \gamma) = \beta \cdot \alpha_1 + \beta \cdot \gamma$. It follows via left cancellation that $0 = \beta \cdot \gamma$. It is then necessary that $\beta = 0$ or $\gamma=0$, but both lead to a contradiction. Hence, $\beta \cdot \alpha_1 = \beta \cdot \alpha_2$ implies $\alpha_1 = \alpha_2$.

    \vspace{1em}

    To prove the converse, we assume that $\alpha_1 = \alpha_2 = \alpha$. But then, it follows by a simple induction on $\alpha$ that $\beta \cdot \alpha_1 = \beta \cdot \alpha = \beta \cdot \alpha_2$.

    
\end{proof}

