\subsection*{3.4} Derive a "parametric" version of the Recursion Theorem (Theorem 3.6) from the Recursion Theorem.

\begin{proof}

The parametric version of the recursion theorem is defined as:

\begin{itemize}
    \item $f(p, 0) = a(p)$ for all $p \in P$
    \item $f(p, n+1) = g(p, f(p,n), n)$ for all $n \in N$ and $p \in P$
\end{itemize}

Define now a function $F: N \rightarrow A$ with

\begin{itemize}
    \item $F(0) = f(p, 0) = a \in A$
    \item $F(n+1) = G(F(n), n) = g(p, F(n), n)$
\end{itemize}

, which is equivalent to the recursion theorem.

\end{proof}

