\subsection*{2.5} Show that, for $n> 0$, $n \cdot 2^{2^{\aleph_0}} = 2^{{\aleph_0}} \cdot 2^{2^{\aleph_0}} = 2^{2^{\aleph_0}} \cdot 2^{2^{\aleph_0}} = (2^{2^{\aleph_0}})^n = (2^{2^{\aleph_0}})^{\aleph_0} = (2^{2^{\aleph_0}})^{2^{\aleph_0}} = 2^{2^{\aleph_0}}$


\begin{proof}
    $$2^{2^{\aleph_0}} \leq n \cdot 2^{2^{\aleph_0}} \leq 2^{n}  \cdot 2^{2^{\aleph_0}} = 2^{2^{\aleph_0}+ n} = 2^{2^{\aleph_0}}$$
    $$2^{2^{\aleph_0}} \leq 2^{{\aleph_0}} \cdot 2^{2^{\aleph_0}} \leq 2^{2^{\aleph_0}} \cdot 2^{2^{\aleph_0}} = 2^{2^{\aleph_0}+2^{\aleph_0}} = 2^{2^{\aleph_0}} $$
    $$2^{2^{\aleph_0}} \leq (2^{2^{\aleph_0}})^n = 2^{n\cdot 2^{\aleph_0}} = 2^{2^{\aleph_0}}$$
    $$(2^{2^{\aleph_0}})^{\aleph_0} = 2^{\aleph_0 \cdot 2^{\aleph_0}} = 2^{2^{\aleph_0}} $$
    $$(2^{2^{\aleph_0}})^{2^{\aleph_0}} = 2^{2^{\aleph_0} \cdot 2^{\aleph_0}} = 2^{2^{\aleph_0}}$$
\end{proof}

