\begin{exercise}{47c}
Show that if $A$ and $B$ are independent, then

$$P(A \cup B) = P(A) + P(B) - P(A)P(B) = 1 - P(A^c)P(B^c)$$
\end{exercise}

\begin{proof}
    If $A$ and $B$ are independent, then $P(A \cap B) = P(A)P(B)$. Substituting this in the formula for the probability of event union, we obtain that

    $$P(A \cup B) = P(A) + P(B) - P(A \cap B) =  P(A) + P(B) - P(A)P(B)$$

    Using the property that $P(A^c) = 1-P(A)$, we have that

    $$P(A^c)P(B^c) = (1-P(A))(1-P(B)) = 1 - P(A) - P(B) + P(A)P(B)$$

    and hence, substituting into the above, we obtain that 

    $$P(A \cup B) = 1 - P(A^c)P(B^c)$$
    
\end{proof}

\newpage

